Working on critical-region-exclusivity

CriticalRegion.v
@@ -3,167 +3,384 @@ From Elo Require Import Core.
 From Elo Require Import WellTypedTerm.
 
 (* ------------------------------------------------------------------------- *)
-(* insideCR                                                                  *)
+(* no-cr & ok-crs                                                            *)
+(* ------------------------------------------------------------------------- *)
+
+Inductive no_cr : tm -> Prop :=
+  | nocr_unit  :                                        no_cr <{unit      }>
+  | nocr_nat   : forall n,                              no_cr <{nat n     }>
+  | nocr_var   : forall x,                              no_cr <{var x     }>
+  | nocr_fun   : forall x Tx t, no_cr t              -> no_cr <{fn x Tx t }>
+  | nocr_call  : forall t1 t2,  no_cr t1 -> no_cr t2 -> no_cr <{call t1 t2}>
+  | nocr_ref   : forall ad T,                           no_cr <{&ad : T   }>
+  | nocr_new   : forall T t,    no_cr t              -> no_cr <{new t : T }>
+  | nocr_load  : forall t,      no_cr t              -> no_cr <{*t        }>
+  | nocr_asg   : forall t1 t2,  no_cr t1 -> no_cr t2 -> no_cr <{t1 := t2  }>
+  | nocr_acq   : forall t1 t2,  no_cr t1 -> no_cr t2 -> no_cr <{acq t1 t2 }>
+  | nocr_spawn : forall t,      no_cr t              -> no_cr <{spawn t   }>
+  .
+
+Inductive ok_crs : tm -> Prop :=
+  | okcrs_unit  :                                          ok_crs <{unit      }>
+  | okcrs_nat   : forall n,                                ok_crs <{nat n     }>
+  | okcrs_var   : forall x,                                ok_crs <{var x     }>
+  | okcrs_fun   : forall x Tx t, no_cr t                -> ok_crs <{fn x Tx t }>
+  | okcrs_call  : forall t1 t2,  ok_crs t1 -> ok_crs t2 -> ok_crs <{call t1 t2}>
+  | okcrs_ref   : forall ad T,                             ok_crs <{&ad : T   }>
+  | okcrs_new   : forall T t,    ok_crs t               -> ok_crs <{new t : T }>
+  | okcrs_load  : forall t,      ok_crs t               -> ok_crs <{*t        }>
+  | okcrs_asg   : forall t1 t2,  ok_crs t1 -> ok_crs t2 -> ok_crs <{t1 := t2  }>
+  | okcrs_acq   : forall t1 t2,  ok_crs t1 -> ok_crs t2 -> ok_crs <{acq t1 t2 }>
+  | okcrs_cr    : forall ad t,   ok_crs t               -> ok_crs <{cr ad t   }>
+  | okcrs_spawn : forall t,      no_cr t                -> ok_crs <{spawn t   }>
+  .
+
+(* inversions -------------------------------------------------------------- *)
+
+Local Ltac _nocr tt :=
+  match goal with
+  | H : no_cr <{unit     }> |- _ => clear H
+  | H : no_cr <{nat _    }> |- _ => clear H
+  | H : no_cr <{var _    }> |- _ => clear H
+  | H : no_cr <{fn _ _ _ }> |- _ => tt H
+  | H : no_cr <{call _ _ }> |- _ => tt H
+  | H : no_cr <{&_ : _   }> |- _ => clear H
+  | H : no_cr <{new _ : _}> |- _ => tt H
+  | H : no_cr <{* _      }> |- _ => tt H
+  | H : no_cr <{_ := _   }> |- _ => tt H
+  | H : no_cr <{acq _ _  }> |- _ => tt H
+  | H : no_cr <{cr _ _   }> |- _ => tt H
+  | H : no_cr <{spawn _  }> |- _ => tt H
+  end.
+
+Local Ltac _okcrs tt :=
+  match goal with
+  | H : ok_crs <{unit     }> |- _ => clear H
+  | H : ok_crs <{nat _    }> |- _ => clear H
+  | H : ok_crs <{var _    }> |- _ => clear H
+  | H : ok_crs <{fn _ _ _ }> |- _ => tt H
+  | H : ok_crs <{call _ _ }> |- _ => tt H
+  | H : ok_crs <{&_ : _   }> |- _ => clear H
+  | H : ok_crs <{new _ : _}> |- _ => tt H
+  | H : ok_crs <{* _      }> |- _ => tt H
+  | H : ok_crs <{_ := _   }> |- _ => tt H
+  | H : ok_crs <{acq _ _  }> |- _ => tt H
+  | H : ok_crs <{cr _ _   }> |- _ => tt H
+  | H : ok_crs <{spawn _  }> |- _ => tt H
+  end.
+
+Ltac inv_nocr  := _nocr inv.
+Ltac invc_nocr := _nocr invc.
+
+Ltac inv_okcrs  := _okcrs inv.
+Ltac invc_okcrs := _okcrs invc.
+
+(* lemmas ------------------------------------------------------------------ *)
+
+Lemma nocr_then_okcrs : forall t,
+  no_cr t ->
+  ok_crs t.
+Proof.
+  intros. induction t; try invc_nocr; eauto using ok_crs.
+Qed.
+
+Lemma value_then_nocr : forall t,
+  value t ->
+  ok_crs t ->
+  no_cr t.
+Proof.
+  intros * Hval **. invc Hval; try invc_okcrs; eauto using no_cr.
+Qed.
+
+(* preservation (valid-crs) ------------------------------------------------ *)
+
+Local Lemma nocr_subst : forall x tx t,
+  no_cr t ->
+  no_cr tx ->
+  no_cr <{[x := tx] t}>.
+Proof.
+  intros. induction t; simpl in *; trivial;
+  try (destruct str_eq_dec; subst); trivial;
+  invc_nocr; eauto using no_cr.
+Qed.
+
+Local Lemma okcrs_subst : forall x tx t,
+  value tx ->
+  no_cr t ->
+  ok_crs tx ->
+  ok_crs <{[x := tx] t}>.
+Proof.
+  intros. induction t; simpl in *; invc_nocr;
+  try (destruct str_eq_dec); eauto using value_then_nocr, nocr_subst, ok_crs.
+Qed.
+
+Local Lemma okcrs_preservation_tm_cstep : forall m1 m2 ths1 ths2 tid e,
+  forall_memory m1 value ->
+  forall_memory m1 ok_crs ->
+  (* --- *)
+  forall_threads ths1 ok_crs ->
+  m1 / ths1 ~~[tid, e]~~> m2 / ths2 ->
+  forall_threads ths2 ok_crs.
+Proof.
+  intros * ? ? H ? tid' **.
+  invc_cstep; try invc_mstep; omicron; trivial;
+  match goal with | _ : _[?tid] --[_]--> _ |- _ => specialize (H tid) end;
+  ind_tstep; repeat invc_okcrs;
+  eauto using okcrs_subst, nocr_then_okcrs, ok_crs.
+Qed.
+
+Local Lemma okcrs_preservation_mem_cstep : forall m1 m2 ths1 ths2 tid e,
+  forall_threads ths1 ok_crs ->
+  (* --- *)
+  forall_memory m1 ok_crs ->
+  m1 / ths1 ~~[tid, e]~~> m2 / ths2 ->
+  forall_memory m2 ok_crs.
+Proof.
+  intros * H ** ?. invc_cstep; try invc_mstep; trivial;
+  omicron; eauto using ok_crs;
+  specialize (H tid); ind_tstep; invc_okcrs; eauto.
+Qed.
+
+Theorem okcrs_preservation : forall m1 m2 ths1 ths2 tid e,
+  forall_memory m1 value ->
+  (* --- *)
+  forall_program m1 ths1 ok_crs ->
+  m1 / ths1 ~~[tid, e]~~> m2 / ths2 ->
+  forall_program m2 ths2 ok_crs.
+Proof.
+  intros * ? [? ?] **. split;
+  eauto using okcrs_preservation_tm_cstep, okcrs_preservation_mem_cstep.
+Qed.
+
+(* ------------------------------------------------------------------------- *)
+(* in-cr                                                                     *)
 (* ------------------------------------------------------------------------- *)
 
 (* Ignores spawn blocks. *)
-Inductive insideCR (ad : addr) : tm -> Prop :=
-  | icr_fun : forall x Tx t,
-    insideCR ad t ->
-    insideCR ad <{fn x Tx t}>
-
-  | icr_call1 : forall t1 t2,
-    insideCR ad t1 ->
-    insideCR ad <{call t1 t2}>
-
-  | icr_call2 : forall t1 t2,
-    insideCR ad t2 ->
-    insideCR ad <{call t1 t2}>
-
-  | icr_new : forall T t,
-    insideCR ad t ->
-    insideCR ad <{new t : T}>
-
-  | icr_load : forall t,
-    insideCR ad t ->
-    insideCR ad <{*t}>
-
-  | icr_asg1 : forall t1 t2,
-    insideCR ad t1 ->
-    insideCR ad <{t1 := t2}>
-
-  | icr_asg2 : forall t1 t2,
-    insideCR ad t2 ->
-    insideCR ad <{t1 := t2}>
-
-  | icr_acq1 : forall t1 t2,
-    insideCR ad t1 ->
-    insideCR ad <{acq t1 t2}>
-
-  | icr_acq2 : forall t1 t2,
-    insideCR ad t2 ->
-    insideCR ad <{acq t1 t2}>
-
-  | icr_cr_eq : forall t,
-    insideCR ad <{cr ad t}>
-
-  | icr_cr_neq : forall ad' t,
-    ad <> ad' ->
-    insideCR ad t ->
-    insideCR ad <{cr ad' t}>
+Inductive in_cr (ad : addr) : tm -> Prop :=
+  | incr_fun   : forall x Tx t, in_cr ad t   -> in_cr ad <{fn x Tx t }>
+  | incr_call1 : forall t1 t2,  in_cr ad t1  -> in_cr ad <{call t1 t2}>
+  | incr_call2 : forall t1 t2,  in_cr ad t2  -> in_cr ad <{call t1 t2}>
+  | incr_new   : forall T t,    in_cr ad t   -> in_cr ad <{new t : T }>
+  | incr_load  : forall t,      in_cr ad t   -> in_cr ad <{*t        }>
+  | incr_asg1  : forall t1 t2,  in_cr ad t1  -> in_cr ad <{t1 := t2  }>
+  | incr_asg2  : forall t1 t2,  in_cr ad t2  -> in_cr ad <{t1 := t2  }>
+  | incr_acq1  : forall t1 t2,  in_cr ad t1  -> in_cr ad <{acq t1 t2 }>
+  | incr_acq2  : forall t1 t2,  in_cr ad t2  -> in_cr ad <{acq t1 t2 }>
+  | incr_eq  : forall t, in_cr ad <{cr ad t}>
+  | incr_neq : forall ad' t, ad <> ad' -> in_cr ad t -> in_cr ad <{cr ad' t}>
   .
 
-(* ------------------------------------------------------------------------- *)
-(* tactics                                                                   *)
-(* ------------------------------------------------------------------------- *)
+(* inversion --------------------------------------------------------------- *)
 
-Local Ltac _icr tt :=
+Local Ltac _incr tt :=
   match goal with
-  | H : insideCR _ <{unit     }> |- _ => tt H
-  | H : insideCR _ <{nat _    }> |- _ => tt H
-  | H : insideCR _ <{var _    }> |- _ => tt H
-  | H : insideCR _ <{fn _ _ _ }> |- _ => tt H
-  | H : insideCR _ <{call _ _ }> |- _ => tt H
-  | H : insideCR _ <{& _ : _  }> |- _ => tt H
-  | H : insideCR _ <{new _ : _}> |- _ => tt H
-  | H : insideCR _ <{* _      }> |- _ => tt H
-  | H : insideCR _ <{_ := _   }> |- _ => tt H
-  | H : insideCR _ <{acq _ _  }> |- _ => tt H
-  | H : insideCR _ <{cr _ _   }> |- _ => tt H
-  | H : insideCR _ <{spawn _  }> |- _ => tt H
+  | H : in_cr _ <{unit     }> |- _ => tt H
+  | H : in_cr _ <{nat _    }> |- _ => tt H
+  | H : in_cr _ <{var _    }> |- _ => tt H
+  | H : in_cr _ <{fn _ _ _ }> |- _ => tt H
+  | H : in_cr _ <{call _ _ }> |- _ => tt H
+  | H : in_cr _ <{& _ : _  }> |- _ => tt H
+  | H : in_cr _ <{new _ : _}> |- _ => tt H
+  | H : in_cr _ <{* _      }> |- _ => tt H
+  | H : in_cr _ <{_ := _   }> |- _ => tt H
+  | H : in_cr _ <{acq _ _  }> |- _ => tt H
+  | H : in_cr _ <{cr _ _   }> |- _ => tt H
+  | H : in_cr _ <{spawn _  }> |- _ => tt H
   end.
 
-Ltac inv_icr  := _icr inv.
-Ltac invc_icr := _icr invc.
+Ltac inv_incr  := _incr inv.
+Ltac invc_incr := _incr invc.
 
-Local Ltac _value tt :=
+(* lemmas ------------------------------------------------------------------ *)
+
+Lemma nocr_then_nincr : forall ad t,
+  no_cr t ->
+  ~ in_cr ad t.
+Proof.
+  intros ** ?. induction t; invc_nocr; invc_incr; eauto.
+Qed.
+
+(* inheritance ------------------------------------------------------------- *)
+
+Local Lemma incr_inheritance_subst : forall ad x Tx t tx,
+  in_cr ad <{[x := tx] t}> ->
+  in_cr ad <{call <{fn x Tx t}> tx}>.
+Proof.
+  intros. induction t; eauto; simpl in *;
+  try (destruct str_eq_dec; subst; eauto using in_cr);
+  invc_incr; repeat auto_specialize; repeat invc_incr; eauto using in_cr.
+Qed.
+
+Local Lemma incr_inheritance_none : forall t1 t2 ad,
+  in_cr ad t2 ->
+  t1 --[e_none]--> t2 ->
+  in_cr ad t1.
+Proof.
+  intros. ind_tstep; try invc_incr; eauto using incr_inheritance_subst, in_cr.
+Qed.
+
+Local Lemma incr_inheritance_alloc : forall t1 t2 ad ad' t T,
+  in_cr ad t2 ->
+  t1 --[e_alloc ad' t T]--> t2 ->
+  in_cr ad t1.
+Proof.
+  intros. ind_tstep; try invc_incr; eauto using in_cr.
+Qed.
+
+Local Lemma incr_inheritance_read : forall t1 t2 ad ad' t,
+  value t ->
+  ok_crs t ->
+  (* --- *)
+  in_cr ad t2 ->
+  t1 --[e_read ad' t]--> t2 ->
+  in_cr ad t1.
+Proof.
+  intros. ind_tstep; try invc_incr; eauto using in_cr.
+  exfalso. eapply nocr_then_nincr; eauto using value_then_nocr.
+Qed.
+
+Local Lemma incr_inheritance_write : forall t1 t2 ad ad' t T,
+  in_cr ad t2 ->
+  t1 --[e_write ad' t T]--> t2 ->
+  in_cr ad t1.
+Proof.
+  intros. ind_tstep; try invc_incr; eauto using in_cr.
+Qed.
+
+Local Lemma incr_inheritance_rel : forall t1 t2 ad ad',
+  ok_crs t1 ->
+  (* --- *)
+  in_cr ad t2 ->
+  t1 --[e_rel ad']--> t2 ->
+  in_cr ad t1.
+Proof.
+  intros. ind_tstep; invc_okcrs; try invc_incr; eauto using in_cr.
+  exfalso. eapply nocr_then_nincr; eauto using value_then_nocr.
+Qed.
+
+Local Lemma incr_inheritance_spawn : forall t1 t2 ad tid t,
+  in_cr ad t2 ->
+  t1 --[e_spawn tid t]--> t2 ->
+  in_cr ad t1.
+Proof.
+  intros. ind_tstep; try invc_incr; eauto using in_cr.
+Qed.
+
+(* preservation ------------------------------------------------------------ *)
+
+Local Lemma incr_subst : forall t tx ad x,
+  in_cr ad t ->
+  in_cr ad <{[x := tx] t}>.
+Proof.
+  intros. induction t; eauto; simpl in *;
+  try (destruct str_eq_dec; subst); invc_incr; eauto using in_cr.
+Qed.
+
+Local Lemma incr_preservation_none : forall t1 t2 ad,
+  ok_crs t1 ->
+  (* --- *)
+  in_cr ad t1 ->
+  t1 --[e_none]--> t2 ->
+  in_cr ad t2.
+Proof.
+  intros. ind_tstep; repeat invc_okcrs; repeat invc_incr;
+  eauto using incr_subst, in_cr.
+  match goal with H : in_cr _ _ |- _ => contradict H end.
+  eauto using value_then_nocr, nocr_then_nincr.
+Qed.
+
+(* ------------------------------------------------------------------------- *)
+(* not-in-cr                                                                 *)
+(* ------------------------------------------------------------------------- *)
+
+Local Ltac solve_inv_nincr := intros; try split; eauto using in_cr.
+
+Local Lemma inv_nincr_fun : forall ad x Tx t,
+  ~ in_cr ad <{fn x Tx t}> -> ~ in_cr ad t.
+Proof. solve_inv_nincr. Qed.
+
+Local Lemma inv_nincr_call : forall ad t1 t2,
+  ~ in_cr ad <{call t1 t2}> -> ~ in_cr ad t1 /\ ~ in_cr ad t2.
+Proof. solve_inv_nincr. Qed.
+
+Local Lemma inv_nincr_new : forall ad t T,
+  ~ in_cr ad <{new t : T}> -> ~ in_cr ad t.
+Proof. solve_inv_nincr. Qed.
+
+Local Lemma inv_nincr_load : forall ad t,
+  ~ in_cr ad <{*t}> -> ~ in_cr ad t.
+Proof. solve_inv_nincr. Qed.
+
+Local Lemma inv_nincr_asg : forall ad t1 t2,
+  ~ in_cr ad <{t1 := t2}> -> ~ in_cr ad t1 /\ ~ in_cr ad t2.
+Proof. solve_inv_nincr. Qed.
+
+Local Lemma inv_nincr_acq : forall ad t1 t2,
+  ~ in_cr ad <{acq t1 t2}> -> ~ in_cr ad t1 /\ ~ in_cr ad t2.
+Proof. solve_inv_nincr. Qed.
+
+Local Lemma inv_nincr_neq : forall ad ad' t,
+  ~ in_cr ad <{cr ad' t}> -> ad <> ad' /\ ~ in_cr ad t.
+Proof.
+  intros * H. split. intros ?.
+  - subst. eauto using in_cr.
+  - intros ?. destruct (nat_eq_dec ad ad'); subst; eauto using in_cr.
+Qed.
+
+Ltac invc_nincr :=
   match goal with
-  (* irrelevant for unit and nat *)
-  | H : value <{var _    }> |- _ => tt H
-  (* irrelevant for function *)
-  | H : value <{call _ _ }> |- _ => tt H
-  (* irrelevant for reference *)
-  | H : value <{new _ : _}> |- _ => tt H
-  | H : value <{* _      }> |- _ => tt H
-  | H : value <{_ := _   }> |- _ => tt H
-  | H : value <{acq _ _  }> |- _ => tt H
-  | H : value <{cr _ _   }> |- _ => tt H
-  | H : value <{spawn _  }> |- _ => tt H
+  | H : ~ in_cr _   <{unit     }> |- _ => clear H
+  | H : ~ in_cr _   <{nat _    }> |- _ => clear H
+  | H : ~ in_cr _   <{var _    }> |- _ => clear H
+  | H : ~ in_cr _   <{fn _ _ _ }> |- _ => eapply inv_nincr_fun    in H
+  | H : ~ in_cr _   <{call _ _ }> |- _ => eapply inv_nincr_call   in H as [? ?]
+  | H : ~ in_cr _   <{& _ : _  }> |- _ => clear H
+  | H : ~ in_cr _   <{new _ : _}> |- _ => eapply inv_nincr_new    in H
+  | H : ~ in_cr _   <{* _      }> |- _ => eapply inv_nincr_load   in H
+  | H : ~ in_cr _   <{_ := _   }> |- _ => eapply inv_nincr_asg    in H as [? ?]
+  | H : ~ in_cr _   <{acq _ _  }> |- _ => eapply inv_nincr_acq    in H as [? ?]
+  | H : ~ in_cr ?ad <{cr ?ad _ }> |- _ => contradict H; eauto using in_cr
+  | H : ~ in_cr _   <{cr _ _   }> |- _ => eapply inv_nincr_neq    in H as [? ?]
+  | H : ~ in_cr _   <{spawn _  }> |- _ => clear H
   end.
 
-Ltac inv_value  := _value inv.
-Ltac invc_value := _value invc.
+(* preservation ------------------------------------------------------------ *)
 
-(* ------------------------------------------------------------------------- *)
-(* value-icr                                                                 *)
-(* ------------------------------------------------------------------------- *)
+Local Lemma nincr_subst : forall ad x tx t,
+  no_cr t ->
+  (* --- *)
+  ~ in_cr ad t ->
+  ~ in_cr ad tx ->
+  ~ in_cr ad <{[x := tx] t}>.
+Proof.
+  intros. induction t; invc_nocr; trivial; simpl in *;
+  try (destruct str_eq_dec; subst); eauto using in_cr;
+  invc_nincr; repeat auto_specialize; intros ?; invc_incr; eauto.
+Qed.
 
-Definition value_icr t := forall ad, value t -> ~ insideCR ad t.
-
-Local Lemma vicr_preservation_none : forall t1 t2,
-  value_icr t1 ->
+Local Lemma nincr_preservation_none : forall t1 t2 ad,
+  ok_crs t1 ->
+  (* --- *)
+  ~ in_cr ad t1 ->
   t1 --[e_none]--> t2 ->
-  value_icr t2.
+  ~ in_cr ad t2.
 Proof.
-  unfold value_icr. intros * Hvicr **.
-  ind_tstep.
-  - invc_value.
-  - invc_value.
-  - admit.
-  - invc_value.
-  - invc_value.
-  - invc_value.
-  - invc_value.
-  - invc_value.
-  - invc_value.
-  - admit.
+  intros. ind_tstep; repeat invc_okcrs; repeat invc_nincr;
+  eauto using nincr_subst;
+  intros ?; invc_incr; eauto;
+  repeat auto_specialize; contradict IHtstep; assumption.
 Qed.
 
-
-(* ------------------------------------------------------------------------- *)
-(* insideCR inheritance                                                          *)
-(* ------------------------------------------------------------------------- *)
-
-Local Lemma icr_inheritance_subst : forall ad x Tx t tx,
-  insideCR ad <{[x := tx] t}> ->
-  insideCR ad <{call <{fn x Tx t}> tx}>.
+Local Lemma nincr_preservation_alloc : forall t1 t2 ad ad' t T,
+  ~ in_cr ad t1 ->
+  t1 --[e_alloc ad' t T]--> t2 ->
+  ~ in_cr ad t2.
 Proof.
-  intros. induction t; eauto; simpl in *;
-  try (destruct str_eq_dec; subst; eauto using insideCR);
-  invc_icr; repeat auto_specialize; repeat invc_icr; eauto using insideCR.
+  intros. ind_tstep; repeat invc_okcrs; repeat invc_nincr;
+  intros ?; invc_incr; eauto;
+  repeat auto_specialize; contradict IHtstep; assumption.
 Qed.
-
-Local Lemma icr_inheritance_none : forall t1 t2 ad,
-  insideCR ad t2 ->
-  t1 --[e_none]--> t2 ->
-  insideCR ad t1.
-Proof.
-  intros. ind_tstep; try invc_icr; eauto using icr_inheritance_subst, insideCR.
-Qed.
-
-(* ------------------------------------------------------------------------- *)
-(* insideCR preservation                                                         *)
-(* ------------------------------------------------------------------------- *)
-
-Local Lemma icr_subst : forall t tx ad x,
-  insideCR ad t ->
-  insideCR ad <{[x := tx] t}>.
-Proof.
-  intros. induction t; eauto; simpl in *;
-  try (destruct str_eq_dec; subst); invc_icr; eauto using insideCR.
-Qed.
-
-Local Lemma icr_preservation_none : forall t1 t2 ad,
-  well_typed_term t1 ->
-  insideCR ad t1 ->
-  t1 --[e_none]--> t2 ->
-  insideCR ad t2.
-Proof.
-  intros. ind_tstep; invc_wtt; repeat invc_icr; eauto using insideCR.
-  - eauto using icr_subst.
-  - invc H0; invc_icr. admit.
-Qed.
-
 
 (* ------------------------------------------------------------------------- *)
 (* invariant                                                                 *)
@@ -171,12 +388,10 @@ Qed.
 
 Definition critical_region_exclusivity (ths : threads) := forall ad tid1 tid2,
   tid1 <> tid2 ->
-  insideCR ad ths[tid1] ->
-  ~ insideCR ad ths[tid2].
+  in_cr ad ths[tid1] ->
+  ~ in_cr ad ths[tid2].
 
-(* ------------------------------------------------------------------------- *)
-(* preservation                                                              *)
-(* ------------------------------------------------------------------------- *)
+(* preservation ------------------------------------------------------------ *)
 
 Local Lemma tstep_length_tid : forall ths tid e t,
   ths[tid] --[e]--> t ->
@@ -192,43 +407,37 @@ Local Ltac destruct_cre ths tid tid1 tid2 :=
   try contradiction.
 
 Local Lemma cre_preservation_none : forall t ths tid,
+  ok_crs ths[tid] ->
+  (* --- *)
   critical_region_exclusivity ths ->
   ths[tid] --[e_none]--> t ->
   critical_region_exclusivity ths[tid <- t].
 Proof.
   unfold critical_region_exclusivity. intros.
-  destruct_cre ths tid tid1 tid2.
-  - sigma. eauto using icr_inheritance_none.
-  - sigma.
+  destruct_cre ths tid tid1 tid2; sigma;
+  eauto using incr_inheritance_none, nincr_preservation_none.
+Qed.
 
-  ind_tstep; intros ? ? ? Hneq Hicr;
-  repeat clean; repeat auto_specialize.
-  - admit.
-  - admit.
-  - admit.
-  - destruct (nat_eq_dec tid1 tid); destruct (nat_eq_dec tid2 tid); subst;
-    sigma; eauto.
-    + invc_icr. specialize (IHtstep ad tid tid2 Hneq). sigma. eauto.
-    + specialize (IHtstep ad tid1 tid Hneq). sigma. intros ?. invc_icr.
-      eapply IHtstep; eauto.
+Local Lemma cre_preservation_alloc : forall t ths tid ad te T,
+  critical_region_exclusivity ths ->
+  ths[tid] --[e_alloc ad te T]--> t ->
+  critical_region_exclusivity ths[tid <- t].
+Proof.
+  unfold critical_region_exclusivity. intros.
+  destruct_cre ths tid tid1 tid2; sigma;
+  eauto using incr_inheritance_alloc, nincr_preservation_alloc.
+Qed.
 
-
-
-
-  - intros ? ? ? Hneq Hicr.
-    repeat clean. repeat auto_specialize.
-    destruct (nat_eq_dec tid1 tid); destruct (nat_eq_dec tid2 tid); subst;
-    sigma; eauto.
-    + admit.
-    +
-
-
-      invc_icr.
-      * specialize (IHtstep ad tid2 tid1 Hneq). sigma.
-        intros ?. eapply IHtstep; eauto.
-      * eapply not_eq_sym in Hneq as Hneq1.
-        specialize (IHtstep ad tid1 tid2 Hneq1) as IH1. sigma.
-        eapply IH1. clear IH1.
-        specialize (IHtstep ad tid2 tid1 Hneq) as IH2. sigma.
-
+Local Lemma cre_preservation_read : forall t ths tid ad te,
+  value te ->
+  ok_crs te ->
+  (* --- *)
+  critical_region_exclusivity ths ->
+  ths[tid] --[e_read ad te]--> t ->
+  critical_region_exclusivity ths[tid <- t].
+Proof.
+  unfold critical_region_exclusivity. intros.
+  destruct_cre ths tid tid1 tid2; sigma;
+  eauto using incr_inheritance_read, nincr_preservation_alloc.
+  admit.
 Qed.
